pulse/src/checker/Pulse.Checker.fst
@@ -376,8 +376,28 @@ let rec check
       | Tm_NuWhile .. -> (
         match post_hint with
         | PostHint _ -> Bind.check_bind g pre pre_typing post_hint res_ppname (seq_with_unit t) check
-        | _ -> While.check_nuwhile g pre pre_typing post_hint res_ppname t check
+        | _ -> While.check_nuwhile g pre pre_typing post_hint res_ppname t (fresh g) None check
       )
+
+      // SUPER HACKY, we pass break invariants from the frontend by annotating a
+      // forward jump label around the while.....
+      | Tm_ForwardJumpLabel { lbl; body = { term = Tm_NuWhile _ }; post } ->
+        if T.unseal lbl.name = "_break" then
+          match post_hint with
+          | PostHint _ ->
+            Bind.check_bind g pre pre_typing post_hint res_ppname (seq_with_unit t) check
+          | _ ->
+            let lblx = fresh g in
+            let Tm_ForwardJumpLabel {body} = t.term in
+            assert Tm_NuWhile? body.term;
+            let body = open_st_term_nv body (lbl, lblx) in
+            assume Tm_NuWhile? body.term;
+            let break_req = match inspect_term (comp_post post) with
+              | Tm_Pure p -> Some p
+              | _ -> None in
+            While.check_nuwhile g pre pre_typing post_hint res_ppname body lblx break_req check
+        else
+          ForwardJumpLabel.check g pre pre_typing post_hint res_ppname t check
 
       | Tm_Match {sc;returns_=post_match;brs} ->
         // TODO : dedup
