pulse/src/checker/Pulse.Checker.While.fsti
@@ -39,5 +39,7 @@ val check_nuwhile
   (post_hint:post_hint_opt g { ~ (PostHint? post_hint) })
   (res_ppname:ppname)
   (t:st_term{Tm_NuWhile? t.term})
+  (break_lbl: var { freshv g break_lbl })
+  (break_inv: option term)
   (check:check_t)
   : T.Tac (checker_result_t g pre post_hint)
