pulse/src/syntax_extension/PulseSyntaxExtension.Sugar.fst
@@ -110,6 +110,7 @@ let ensures_slprop = option (ident & A.term) & slprop & option A.term
 type while_invariant1 =
   | Old of ident & slprop
   | New of slprop
+  | BreakRequires of A.term
 
 type while_invariant = list while_invariant1
 
@@ -192,6 +193,7 @@ type stmt' =
 
   | Return { arg: option A.term }
   | Continue
+  | Break
 
 and stmt = {
   s:stmt';
@@ -282,7 +284,9 @@ instance showable_a_binder : showable A.binder = {
 instance showable_while_invariant1 : showable while_invariant1 = {
   show = (fun i -> match i with
     | Old x -> "Old " ^ show x
-    | New x -> "New " ^ show x);
+    | New x -> "New " ^ show x
+    | BreakRequires x -> "BreakRequires " ^ show x
+    );
 }
 
 let rec stmt_to_string (s:stmt) : string =
@@ -381,6 +385,7 @@ let eq_while_invariant1 (i1 i2:while_invariant1) =
   match i1, i2 with
   | Old (id1, t1), Old (id2, t2) -> eq_ident id1 id2 && eq_slprop t1 t2
   | New t1, New t2 -> eq_slprop t1 t2
+  | BreakRequires t1, BreakRequires t2 -> AD.eq_term t1 t2
   | _, _ -> false
 
 let rec eq_decl (d1 d2:decl) =
@@ -469,6 +474,8 @@ and eq_stmt' (s1 s2:stmt') =
   | Return { arg=a1 }, Return { arg=a2 } ->
     eq_opt AD.eq_term a1 a2
   | Continue, Continue ->
+    true
+  | Break, Break ->
     true
   | _ -> false
 and eq_let_init (i1 i2:let_init) =
@@ -564,6 +571,7 @@ and scan_while_invariant1 (cbs:A.dep_scan_callbacks) (i:while_invariant1) =
   match i with
   | Old (id, t) -> cbs.scan_term t
   | New t -> cbs.scan_term t
+  | BreakRequires t -> cbs.scan_term t
 and scan_stmt (cbs:A.dep_scan_callbacks) (s:stmt) =
   match s.s with
   | Open l -> cbs.add_open l
@@ -604,6 +612,8 @@ and scan_stmt (cbs:A.dep_scan_callbacks) (s:stmt) =
   | Return { arg } ->
     iopt cbs.scan_term arg
   | Continue ->
+    ()
+  | Break ->
     ()
 and scan_let_init (cbs:A.dep_scan_callbacks) (i:let_init) =
   match i with
@@ -670,3 +680,4 @@ let mk_forward_jump_label body lbl post = ForwardJumpLabel { body; lbl; post }
 let mk_goto lbl arg = Goto { lbl; arg }
 let mk_return arg = Return { arg }
 let mk_continue = Continue
+let mk_break = Break
