pulse/test/Break.fst
@@ -1,0 +1,39 @@
+module Break
+open Pulse
+open Pulse.Lib.WithPure
+#lang-pulse
+
+fn simple_break ()
+{
+  let mut k = true;
+  while (!k)
+    invariant live k
+    break requires true
+  {
+    break;
+  }
+}
+
+fn find_zero_with_break (a: array Int32.t) (sz: SizeT.t)
+  preserves pts_to a #'r 'va
+  requires with_pure (SizeT.v sz <= Seq.length 'va)
+  returns i: SizeT.t
+  ensures pure (SizeT.v i <= SizeT.v sz /\
+    (forall (j: nat). j < SizeT.v i ==> Seq.index 'va j <> 0l))
+  ensures pure (SizeT.v i < SizeT.v sz ==> Seq.index 'va (SizeT.v i) == 0l)
+{
+  let mut i: SizeT.t = 0sz;
+  while (!i `SizeT.lt` sz)
+    invariant live i
+    invariant pure (SizeT.v !i <= SizeT.v sz /\
+      (forall (j: nat). j < SizeT.v (!i) ==> Seq.index 'va j <> 0l))
+    break requires (SizeT.v !i < SizeT.v sz /\ a.(!i) = 0l)
+  {
+    if (a.(!i) = 0l) {
+      break;
+    };
+
+    i := !i `SizeT.add` 1sz;
+  };
+  !i
+}
